Finished converting modules to records in Patterns.
Had to change some theorem names to resolve namespace conflicts.

src/Spec/Patterns.v
@@ -31,14 +31,14 @@ Section TraceAbs.
   ts2, relating them to a compiled version using low-level operations that we
   can actually execute) *)
   Definition traces_match_abs
-                           (ts1 : threads_state OpLo)
-                           (ts2 : threads_state OpHi) :=
+             (ts1 : threads_state OpLo)
+             (ts2 : threads_state OpHi) :=
     forall (sl : StateLo) tr1,
       initP sl ->
       exec lo_step sl ts1 tr1 ->
       exists sm, absR sl sm /\
-            initHi sm /\
-            exec hi_step sm ts2 tr1.
+                 initHi sm /\
+                 exec hi_step sm ts2 tr1.
 
 End TraceAbs.
 
@@ -55,7 +55,7 @@ Module LayerImpl.
       `(l1 : Layer O1 S1)
       `(l2 : Layer O2 S2).
 
-    Record T :=
+    Record t :=
       { absR : S1 -> S2 -> Prop;
         compile_ts : threads_state O2 -> threads_state O1;
         compile_ts_no_atomics :
@@ -66,7 +66,7 @@ Module LayerImpl.
           forall s1,
             l1.(initP) s1 ->
             exists s2, absR s1 s2 /\
-                  l2.(initP) s2;
+                       l2.(initP) s2;
         compile_traces_match :
           forall ts,
             no_atomics_ts ts ->
@@ -81,12 +81,12 @@ Module LayerImplAbsT.
             `(l1: Layer O S1)
             `(l2: Layer O S2).
 
-    Record T :=
+    Record t :=
       { absR : S1 -> S2 -> Prop;
         absR_ok : op_abs absR l1.(step) l2.(step);
         absInitP :
           forall s1, l1.(initP) s1 ->
-                exists s2, absR s1 s2 /\ l2.(initP) s2; }.
+                     exists s2, absR s1 s2 /\ l2.(initP) s2; }.
   End S.
 
 End LayerImplAbsT.
@@ -98,7 +98,7 @@ Module LayerImplAbs.
     Context O
             `(l1 : Layer O S1)
             `(l2 : Layer O S2)
-            (a : LayerImplAbsT.T l1 l2).
+            (a : LayerImplAbsT.t l1 l2).
 
     Definition absR := a.(absR).
     Definition absInitP := a.(absInitP).
@@ -124,7 +124,7 @@ Module LayerImplAbs.
       eapply absInitP in H0; propositional; eauto using trace_incl_abs.
     Qed.
 
-    Definition t : LayerImpl.T l1 l2.
+    Definition t : LayerImpl.t l1 l2.
       refine {| LayerImpl.absR := absR;
                 LayerImpl.absInitP := absInitP;
                 LayerImpl.compile_ts := compile_ts;
@@ -136,26 +136,22 @@ Module LayerImplAbs.
 
 End LayerImplAbs.
 
+Module LayerImplMoversT.
+  Section S.
+    Context S
+            `(l1: Layer O1 S)
+            `(l2: Layer O2 S).
+    Record t :=
+      { compile_op : forall T, O2 T -> proc O1 T;
+        compile_op_no_atomics : forall T (op : O2 T),
+            no_atomics (compile_op op);
+        ysa_movers : forall T (op : O2 T), ysa_movers l1.(step) (compile_op op);
+        compile_correct : compile_correct compile_op l1.(step) l2.(step);
+        initP_compat : forall s, l1.(initP) s -> l2.(initP) s;
+      }.
 
-Module Type LayerImplMoversT
-  (s : State)
-  (o1 : Ops) (l1 : Layer o1 s)
-  (o2 : Ops) (l2 : Layer o2 s).
-
-  Axiom compile_op : forall T, o2.Op T -> proc o1.Op T.
-
-  Axiom compile_op_no_atomics : forall T (op : o2.Op T),
-    no_atomics (compile_op op).
-
-  Axiom ysa_movers : forall T (op : o2.Op T),
-    ysa_movers l1.step (compile_op op).
-
-  Axiom compile_correct :
-    compile_correct compile_op l1.step l2.step.
-
-  Axiom initP_compat : forall s,
-      l1.initP s -> l2.initP s.
-
+  End S.
+  Arguments compile_op [S] {O1} [l1] {O2} [l2] _ [T] op.
 End LayerImplMoversT.
 
 Local Ltac init_abs :=
@@ -167,464 +163,441 @@ Local Ltac init_abs :=
            eexists; split; [ reflexivity | ]
          end.
 
-Module LayerImplMovers
-  (s : State)
-  (o1 : Ops) (l1 : Layer o1 s)
-  (o2 : Ops) (l2 : Layer o2 s)
-  (a : LayerImplMoversT s o1 l1 o2 l2) <: LayerImpl o1 s l1 o2 s l2.
 
-  Definition absR (s1 : s.State) (s2 : s.State) := s1 = s2.
+Module LayerImplMovers.
+  Import LayerImplMoversT.
+  Section S.
+    Context S
+            `(l1 : Layer O1 S)
+            `(l2 : Layer O2 S)
+            (a : LayerImplMoversT.t l1 l2).
 
-  Theorem absInitP :
-    forall s1,
-      l1.initP s1 ->
-      exists s2, absR s1 s2 /\
-            l2.initP s2.
-  Proof.
-    init_abs; auto using a.initP_compat.
-  Qed.
+    Definition absR (s1 : S) (s2: S) := s1 = s2.
+    
+    Theorem absInitP :
+      forall s1,
+        l1.(initP) s1 ->
+        exists s2, absR s1 s2 /\
+                   l2.(initP) s2.
+    Proof.
+      init_abs; auto using a.(initP_compat).
+    Qed.
 
+    Definition compile_ts := Compile.compile_ts a.(compile_op).
 
-  Definition compile_ts := Compile.compile_ts a.compile_op.
+    Theorem compile_ts_no_atomics :
+      forall ts,
+        no_atomics_ts ts ->
+        no_atomics_ts (compile_ts ts).
+    Proof.
+      eapply Compile.compile_ts_no_atomics.
+      eapply a.(compile_op_no_atomics).
+    Qed.
 
-  Theorem compile_ts_no_atomics :
-    forall ts,
-      no_atomics_ts ts ->
-      no_atomics_ts (compile_ts ts).
-  Proof.
-    eapply Compile.compile_ts_no_atomics.
-    eapply a.compile_op_no_atomics.
-  Qed.
+    Check a.(compile_op).
 
-  Theorem op_atomic : forall `(op : o2.Op T) `(rx : _ -> proc _ R),
-    trace_incl l1.step
-      (Bind (a.compile_op op) rx)
-      (Bind (atomize a.compile_op op) rx).
-  Proof.
-    intros.
-    eapply trace_incl_atomize_ysa.
-    eapply a.ysa_movers.
-  Qed.
+    Theorem op_atomic : forall T (op : O2 T) `(rx : _ -> proc _ R),
+        trace_incl l1.(step)
+                        (Bind (a.(compile_op) op) rx)
+                        (Bind (atomize a.(compile_op) op) rx).
+    Proof.
+      intros.
+      eapply trace_incl_atomize_ysa.
+      eapply a.(ysa_movers).
+    Qed.
 
-  Theorem atomize_correct :
-    atomize_correct a.compile_op l1.step.
-  Proof.
-    unfold atomize_correct; intros.
-    rewrite op_atomic.
-    eapply trace_incl_bind_a.
-    eauto.
-  Qed.
+    Theorem atomize_correct :
+      atomize_correct a.(compile_op) l1.(step).
+    Proof.
+      unfold atomize_correct; intros.
+      rewrite op_atomic.
+      eapply trace_incl_bind_a.
+      eauto.
+    Qed.
 
-  Hint Resolve a.compile_correct.
-  Hint Resolve atomize_correct.
+    Hint Resolve atomize_correct.
 
-  Theorem all_traces_match :
-    forall ts1 ts2,
-      proc_match (Compile.compile_ok a.compile_op) ts1 ts2 ->
-      traces_match_ts l1.step l2.step ts1 ts2.
-  Proof.
-    intros.
-    eapply Compile.compile_traces_match_ts; eauto.
-  Qed.
+    Theorem all_traces_match :
+      forall ts1 ts2,
+        proc_match (Compile.compile_ok a.(compile_op)) ts1 ts2 ->
+        traces_match_ts l1.(step) l2.(step) ts1 ts2.
+    Proof.
+      intros.
+      eapply Compile.compile_traces_match_ts; eauto.
+      eapply a.(compile_correct).
+    Qed.
 
-  Theorem compile_traces_match :
-    forall ts2,
-      no_atomics_ts ts2 ->
-      traces_match_abs absR l1.initP l2.initP l1.step l2.step (compile_ts ts2) ts2.
-  Proof.
-    unfold traces_match_abs; intros.
-    init_abs.
-    intuition auto using a.initP_compat.
-    eapply all_traces_match; eauto.
-    eapply Compile.compile_ts_ok; eauto.
-  Qed.
-
+    Theorem compile_traces_match :
+      forall ts2,
+        no_atomics_ts ts2 ->
+        traces_match_abs absR l1.(initP) l2.(initP) l1.(step) l2.(step) (compile_ts ts2) ts2.
+    Proof.
+      unfold traces_match_abs; intros.
+      init_abs.
+      intuition auto using a.(initP_compat).
+      eapply all_traces_match; eauto.
+      eapply Compile.compile_ts_ok; eauto.
+    Qed.
+  End S.
 End LayerImplMovers.
 
+Module LayerImplMoversProtocolT.
+  Import LayerImplMoversT.
+  Section S.
+    Context S
+            `(l1raw: Layer O1 S) (l1: Layer O1 S)
+            `(l2: Layer O2 S)
+            (p: Protocol O1 S).
 
-Module Type LayerImplRequiresRule
-       (o1: Ops) (s1: State) (l1: Layer o1 s1)
-       (o2: Ops) (s2: State) (l2: Layer o2 s2)
-       (p: Protocol o2 s2).
-
-  Axiom absR : s1.State -> s2.State -> Prop.
-  Axiom compile_ts : threads_state o2.Op -> threads_state o1.Op.
-  Axiom compile_ts_no_atomics :
-    forall ts,
-      no_atomics_ts ts ->
-      no_atomics_ts (compile_ts ts).
-  Axiom absInitP :
-    forall s1,
-      l1.initP s1 -> exists s2, absR s1 s2 /\ l2.initP s2.
-  Axiom compile_traces_match :
-    forall ts,
-      no_atomics_ts ts ->
-      (forall s, follows_protocol_s l2.step p.step_allow ts s) ->
-      traces_match_abs absR l1.initP l2.initP l1.step l2.step (compile_ts ts) ts.
-End LayerImplRequiresRule.
-
-
-Module Type LayerImplFollowsRule
-       (o1: Ops) (s1: State) (l1: Layer o1 s1)
-       (o2: Ops) (s2: State) (l2: Layer o2 s2)
-       (p: Protocol o2 s2).
-
-End LayerImplFollowsRule.
-
-
-Module Type LayerImplMoversProtocolT
-  (s : State)
-  (o1 : Ops) (l1raw : Layer o1 s) (l1 : Layer o1 s)
-  (o2 : Ops) (l2 : Layer o2 s)
-  (p : Protocol o1 s).
-
-  Include (LayerImplMoversT s o1 l1 o2 l2).
-
-  Axiom op_follows_protocol : forall tid s `(op : o2.Op T),
-    follows_protocol_proc l1raw.step p.step_allow tid s (compile_op op).
-
-  Axiom allowed_stable :
-    forall `(op : o1.Op T) `(op' : o1.Op T') tid tid' s s' r evs,
-      tid <> tid' ->
-      p.step_allow op tid s ->
-      l1.step op' tid' s r s' evs ->
-      p.step_allow op tid s'.
-
-  (* This means that l1.step is either restricted_step or nilpotent_step *)
-  Axiom raw_step_ok :
-    forall `(op : o1.Op T) tid s r s' evs,
-      restricted_step l1raw.step p.step_allow op tid s r s' evs ->
-      l1.step op tid s r s' evs.
-
-  Axiom raw_initP_compat :
-    forall s, l1raw.initP s -> l1.initP s.
-
+    Record t : Type :=
+      { movers_impl :> LayerImplMoversT.t l1 l2;
+        op_follows_protocol : forall tid S T (op : O2 T),
+            follows_protocol_proc l1raw.(step) p.(step_allow) tid S (movers_impl.(compile_op) op);
+        allowed_stable : 
+          forall T (op : O1 T) T' (op' : O1 T') tid tid' S S' r evs,
+            tid <> tid' ->
+            p.(step_allow) T op tid S ->
+            l1.(step) op' tid' S r S' evs ->
+            p.(step_allow) T op tid S';
+        (* This means that l1.step is either restricted_step or nilpotent_step *)
+        raw_step_ok : 
+          forall T (op : O1 T) tid S r S' evs,
+            restricted_step l1raw.(step) p.(step_allow) op tid S r S' evs ->
+            l1.(step) op tid S r S' evs;
+        raw_initP_compat : forall S, l1raw.(initP) S -> l1.(initP) S;
+      }.
+  End S.
 End LayerImplMoversProtocolT.
 
+Module LayerImplMoversProtocol.
+  Export LayerImplMoversT.
+  Export LayerImplMoversProtocolT.
+  
+  Section S.
+    Context S
+            `(l1raw : Layer O1 S) (l1: Layer O1 S)
+            `(l2 : Layer O2 S)
+            (p : Protocol O1 S)
+            (a : LayerImplMoversProtocolT.t l1raw l1 l2 p).
 
-Module LayerImplMoversProtocol
-  (s : State)
-  (o1 : Ops) (l1raw : Layer o1 s) (l1 : Layer o1 s)
-  (o2 : Ops) (l2 : Layer o2 s)
-  (p : Protocol o1 s)
-  (a : LayerImplMoversProtocolT s o1 l1raw l1 o2 l2 p) <: LayerImpl o1 s l1raw o2 s l2.
+    Definition absR (s1 : S) (s2 : S) := s1 = s2.
 
-  Definition absR (s1 : s.State) (s2 : s.State) := s1 = s2.
+    Theorem absInitP :
+      forall s1,
+        l1raw.(initP) s1 ->
+        exists s2, absR s1 s2 /\
+                   l2.(initP) s2.
+    Proof.
+      unfold absR; init_abs; auto using a.(initP_compat), a.(raw_initP_compat).
+    Qed.
 
-  Theorem absInitP :
-    forall s1,
-      l1raw.initP s1 ->
-      exists s2, absR s1 s2 /\
-      l2.initP s2.
-  Proof.
-    unfold absR; init_abs; auto using a.initP_compat, a.raw_initP_compat.
-  Qed.
+    Definition compile_ts := Compile.compile_ts a.(compile_op).
 
+    Theorem compile_ts_no_atomics :
+      forall ts,
+        no_atomics_ts ts ->
+        no_atomics_ts (compile_ts ts).
+    Proof.
+      eapply Compile.compile_ts_no_atomics.
+      eapply a.(compile_op_no_atomics).
+    Qed.
 
-  Definition compile_ts := Compile.compile_ts a.compile_op.
+    Theorem op_atomic : forall T (op : O2 T) `(rx : _ -> proc _ R),
+        trace_incl l1.(step)
+                        (Bind (a.(compile_op) op) rx)
+                        (Bind (atomize a.(compile_op) op) rx).
+    Proof.
+      intros.
+      eapply trace_incl_atomize_ysa.
+      eapply a.(ysa_movers).
+    Qed.
 
-  Theorem compile_ts_no_atomics :
-    forall ts,
-      no_atomics_ts ts ->
-      no_atomics_ts (compile_ts ts).
-  Proof.
-    eapply Compile.compile_ts_no_atomics.
-    eapply a.compile_op_no_atomics.
-  Qed.
+    Theorem atomize_correct :
+      atomize_correct a.(compile_op) l1.(step).
+    Proof.
+      unfold atomize_correct; intros.
+      rewrite op_atomic.
+      eapply trace_incl_bind_a.
+      eauto.
+    Qed.
 
-  Theorem op_atomic : forall `(op : o2.Op T) `(rx : _ -> proc _ R),
-    trace_incl l1.step
-      (Bind (a.compile_op op) rx)
-      (Bind (atomize a.compile_op op) rx).
-  Proof.
-    intros.
-    eapply trace_incl_atomize_ysa.
-    eapply a.ysa_movers.
-  Qed.
+    Hint Resolve atomize_correct.
 
-  Theorem atomize_correct :
-    atomize_correct a.compile_op l1.step.
-  Proof.
-    unfold atomize_correct; intros.
-    rewrite op_atomic.
-    eapply trace_incl_bind_a.
-    eauto.
-  Qed.
+    Theorem all_traces_match :
+      forall ts1 ts2,
+        proc_match (Compile.compile_ok a.(compile_op)) ts1 ts2 ->
+        traces_match_ts l1.(step) l2.(step) ts1 ts2.
+    Proof.
+      intros.
+      eapply Compile.compile_traces_match_ts; eauto.
+      eapply a.(compile_correct).
+    Qed.
 
-  Hint Resolve a.compile_correct.
-  Hint Resolve atomize_correct.
+    Theorem compile_traces_match_l1 :
+      forall ts2,
+        no_atomics_ts ts2 ->
+        traces_match_abs absR l1.(initP) l2.(initP) l1.(step) l2.(step) (compile_ts ts2) ts2.
+    Proof.
+      unfold traces_match_abs; init_abs.
+      intuition auto using a.(initP_compat).
+      eapply all_traces_match; eauto.
+      eapply Compile.compile_ts_ok; eauto.
+    Qed.
 
-  Theorem all_traces_match :
-    forall ts1 ts2,
-      proc_match (Compile.compile_ok a.compile_op) ts1 ts2 ->
-      traces_match_ts l1.step l2.step ts1 ts2.
-  Proof.
-    intros.
-    eapply Compile.compile_traces_match_ts; eauto.
-  Qed.
+    Definition follows_protocol (ts : threads_state O1) :=
+      forall s,
+        follows_protocol_s l1raw.(step) p.(step_allow) ts s.
 
-  Theorem compile_traces_match_l1 :
-    forall ts2,
-      no_atomics_ts ts2 ->
-      traces_match_abs absR l1.initP l2.initP l1.step l2.step (compile_ts ts2) ts2.
-  Proof.
-    unfold traces_match_abs; init_abs.
-    intuition auto using a.initP_compat.
-    eapply all_traces_match; eauto.
-    eapply Compile.compile_ts_ok; eauto.
-  Qed.
+    Theorem compile_ts_follows_protocol :
+      forall ts,
+        no_atomics_ts ts ->
+        follows_protocol (Compile.compile_ts a.(compile_op) ts).
+    Proof.
+      unfold follows_protocol.
+      unfold follows_protocol_s.
+      intros.
+      eapply compile_ts_follows_protocol_proc; try eassumption.
+      intros.
 
-  Definition follows_protocol (ts : threads_state o1.Op) :=
-    forall s,
-      follows_protocol_s l1raw.step p.step_allow ts s.
+      eapply a.(op_follows_protocol).
+    Qed.
 
-  Theorem compile_ts_follows_protocol :
-    forall ts,
-      no_atomics_ts ts ->
-      follows_protocol (Compile.compile_ts a.compile_op ts).
-  Proof.
-    unfold follows_protocol.
-    unfold follows_protocol_s.
-    intros.
-    eapply compile_ts_follows_protocol_proc; try eassumption.
-    intros.
-
-    eapply a.op_follows_protocol.
-  Qed.
-
-  Lemma follows_protocol_s_spawn:
-    forall (ts : threads_state _) (s : s.State) (T : Type) (tid tid' : nat)
-      (p : proc o1.Op T) (s' : s.State) (evs : list event)
-      (result : T + proc o1.Op T) (spawned : maybe_proc o1.Op),
-      tid <> tid' ->
-      ts tid' = NoProc ->
-      follows_protocol_s l1raw.step p.step_allow ts s ->
-      exec_tid l1raw.step tid s p s' result spawned evs ->
-      follows_protocol_proc l1raw.step p.step_allow tid s p ->
-      follows_protocol_s l1raw.step p.step_allow (ts [[tid' := spawned]]) s.
-  Proof.
-    intros.
-    destruct spawned; cycle 1.
-    rewrite thread_upd_same_eq with (tid:=tid') in * by auto; eauto.
-    unfold follows_protocol_s; intros.
-    cmp_ts tid0 tid'; repeat maybe_proc_inv; eauto.
-    remember (Proc p1).
-    generalize dependent p1.
-    generalize dependent tid'.
-    induction H2; propositional; eauto; NoProc_upd;
-      repeat maybe_proc_inv.
-    invert H3.
-    eapply IHexec_tid; eauto.
-    invert H3; eauto.
-  Qed.
-
-  Lemma no_atomics_ts_exec_spawn:
-    forall (ts : threads_state _) (s : s.State),
-      no_atomics_ts ts ->
-      forall (T : Type) (tid tid' : nat) (p : proc o1.Op T) (s' : s.State)
-        (evs : list event) (result : T + proc o1.Op T) (T0 : Type)
-        (p0 : proc o1.Op T0),
-        ts tid = Proc p ->
-        exec_tid l1raw.step tid s p s' result (Proc p0) evs ->
-        no_atomics_ts (ts [[tid' := Proc p0]]).
-  Proof.
-    intros.
-    eapply no_atomics_thread_upd_Proc; auto.
-    assert (no_atomics p).
-    unfold no_atomics_ts in H0.
-    eapply thread_Forall_some with (a:=tid) in H0; eauto.
-    clear dependent ts.
-
-    (* goal is now simplified to just be about one process *)
-    remember (Proc p0).
-    generalize dependent p0.
-    induction H1; intros; repeat maybe_proc_inv; propositional.
-    invert H2; eauto.
-    invert H2.
-  Qed.
-
-  Theorem compile_traces_match_l1raw :
-    forall ts,
-      follows_protocol ts ->
-      no_atomics_ts ts ->
-      traces_match_abs absR l1raw.initP l1.initP l1raw.step l1.step ts ts.
-  Proof.
-    unfold compile_ts, follows_protocol, absR.
-    unfold traces_match_abs; intros; subst.
-    init_abs.
-    intuition auto using a.raw_initP_compat.
-    clear H1.
-    specialize (H sl).
-    induction H2; eauto.
-    cmp_ts tid tid'.
-    pose proof (H tid _ p ltac:(eauto)) as Htid.
-
-    prove_hyps IHexec.
-    - eapply follows_protocol_s_exec_tid_upd; eauto.
-      intros; eapply a.allowed_stable; eauto.
-      eapply a.raw_step_ok; eauto.
-
-      destruct spawned.
-      eauto using follows_protocol_s_spawn.
+    Lemma follows_protocol_s_spawn:
+      forall (ts : threads_state _) (s : S) (T : Type) (tid tid' : nat)
+             (p0 : proc O1 T) (s' : S) (evs : list event)
+             (result : T + proc O1 T) (spawned : maybe_proc O1),
+        tid <> tid' ->
+        ts tid' = NoProc ->
+        follows_protocol_s l1raw.(step) p.(step_allow) ts s ->
+        exec_tid l1raw.(step) tid s p0 s' result spawned evs ->
+        follows_protocol_proc l1raw.(step) p.(step_allow) tid s p0 ->
+        follows_protocol_s l1raw.(step) p.(step_allow) (ts [[tid' := spawned]]) s.
+    Proof.
+      intros.
+      destruct spawned; cycle 1.
       rewrite thread_upd_same_eq with (tid:=tid') in * by auto; eauto.
+      unfold follows_protocol_s; intros.
+      cmp_ts tid0 tid'; repeat maybe_proc_inv; eauto.
+      remember (Proc p2).
+      generalize dependent p2.
+      generalize dependent tid'.
+      induction H2; propositional; eauto; NoProc_upd;
+        repeat maybe_proc_inv.
+      invert H3.
+      eapply IHexec_tid; eauto.
+      invert H3; eauto.
+    Qed.
 
-      autorewrite with t; auto.
+    Lemma no_atomics_ts_exec_spawn:
+      forall (ts : threads_state _) (s : S),
+        no_atomics_ts ts ->
+        forall (T : Type) (tid tid' : nat) (p0 : proc O1 T) (s' : S)
+               (evs : list event) (result : T + proc O1 T) (T0 : Type)
+               (p1 : proc O1 T0),
+          ts tid = Proc p0 ->
+          exec_tid l1raw.(step) tid s p0 s' result (Proc p1) evs ->
+          no_atomics_ts (ts [[tid' := Proc p1]]).
+    Proof.
+      intros.
+      eapply no_atomics_thread_upd_Proc; auto.
+      assert (no_atomics p0).
+      unfold no_atomics_ts in H.
+      eapply thread_Forall_some with (a:=tid) in H; eauto.
+      clear dependent ts.
 
-      destruct spawned; eauto using no_atomics_ts_exec_spawn,
-                        no_atomics_thread_upd_NoProc.
-    - destruct spawned.
-      destruct matches; eauto using no_atomics_ts_exec_spawn.
-      rewrite thread_upd_same_eq with (tid:=tid') in * by auto;
-        destruct matches;
-        eauto.
-    - ExecPrefix tid tid'.
-      eapply exec_tid_step_impl.
-      intros; apply a.raw_step_ok; eauto.
-      eapply follows_protocol_preserves_exec_tid'; eauto.
-  Qed.
+      (* goal is now simplified to just be about one process *)
+      remember (Proc p1).
+      generalize dependent p1.
+      induction H1; intros; repeat maybe_proc_inv; propositional.
+      invert H2; eauto.
+      invert H2.
+    Qed.
 
-  Hint Resolve (_:Reflexive absR).
-  Local Hint Resolve (_:Transitive absR).
+    Theorem compile_traces_match_l1raw :
+      forall ts,
+        follows_protocol ts ->
+        no_atomics_ts ts ->
+        traces_match_abs absR l1raw.(initP) l1.(initP) l1raw.(step) l1.(step) ts ts.
+    Proof.
+      unfold compile_ts, follows_protocol, absR.
+      unfold traces_match_abs; intros; subst.
+      init_abs.
+      intuition auto using a.(raw_initP_compat).
+      clear H1.
+      specialize (H sl).
+      induction H2; eauto.
+      cmp_ts tid tid'.
+      pose proof (H tid _ p0 ltac:(eauto)) as Htid.
 
-  Local Hint Resolve compile_ts_no_atomics.
-  Local Hint Resolve compile_ts_follows_protocol.
-  Local Hint Resolve a.compile_op_no_atomics.
+      prove_hyps IHexec.
+      - eapply follows_protocol_s_exec_tid_upd; eauto.
+        intros; eapply a.(allowed_stable); eauto.
+        eapply a.(raw_step_ok); eauto.
 
-  Theorem compile_traces_match :
-    forall ts,
-      no_atomics_ts ts ->
-      traces_match_abs absR l1raw.initP l2.initP l1raw.step l2.step (compile_ts ts) ts.
-  Proof.
-    unfold traces_match_abs; intros.
-    eapply compile_traces_match_l1raw in H1; propositional; eauto.
-    eapply compile_traces_match_l1 in H3; propositional; eauto.
-  Qed.
+        destruct spawned.
+        eauto using follows_protocol_s_spawn.
+        rewrite thread_upd_same_eq with (tid:=tid') in * by auto; eauto.
 
-  Theorem initP_compat : forall s,
-      l1raw.initP s -> l2.initP s.
-  Proof.
-    auto using a.initP_compat, a.raw_initP_compat.
-  Qed.
+        autorewrite with t; auto.
 
+        destruct spawned; eauto using no_atomics_ts_exec_spawn,
+                          no_atomics_thread_upd_NoProc.
+      - destruct spawned.
+        destruct matches; eauto using no_atomics_ts_exec_spawn.
+        rewrite thread_upd_same_eq with (tid:=tid') in * by auto;
+          destruct matches;
+          eauto.
+      - ExecPrefix tid tid'.
+        eapply exec_tid_step_impl.
+        intros; apply a.(raw_step_ok); eauto.
+        eapply follows_protocol_preserves_exec_tid'; eauto.
+    Qed.
+
+    Hint Resolve (_:Reflexive absR).
+    Local Hint Resolve (_:Transitive absR).
+
+    Local Hint Resolve compile_ts_no_atomics.
+    Local Hint Resolve compile_ts_follows_protocol.
+
+    Theorem compile_traces_match :
+      forall ts,
+        no_atomics_ts ts ->
+        traces_match_abs absR l1raw.(initP) l2.(initP) l1raw.(step) l2.(step) (compile_ts ts) ts.
+    Proof.
+      unfold traces_match_abs; intros.
+      eapply compile_traces_match_l1raw in H1; propositional; eauto.
+      eapply compile_traces_match_l1 in H3; propositional; eauto.
+    Qed.
+
+    Theorem initP_compat : forall s,
+        l1raw.(initP) s -> l2.(initP) s.
+    Proof.
+      auto using a.(initP_compat), a.(raw_initP_compat).
+    Qed.
+
+  End S.
 End LayerImplMoversProtocol.
 
+Module LayerImplLoopT.
+  Section S.
+    Context S
+            `(l1: Layer O1 S)
+            `(l2: Layer O2 S).
 
-Module Type LayerImplLoopT
-  (s : State)
-  (o1 : Ops) (l1 : Layer o1 s)
-  (o2 : Ops) (l2 : Layer o2 s).
-
-  Axiom compile_op : forall T, o2.Op T -> (option T -> o1.Op T) * (T -> bool) * option T.
-  Axiom noop_or_success :
-    noop_or_success compile_op l1.step l2.step.
-
-  Axiom initP_compat :
-    forall s, l1.initP s -> l2.initP s.
-
+    Record t :=
+      { compile_op : forall T, O2 T -> (option T -> O1 T) * (T -> bool) * option T;
+        noop_or_success : noop_or_success compile_op l1.(step) l2.(step);
+        initP_compat : forall s, l1.(initP) s -> l2.(initP) s; }.
+  End S.
 End LayerImplLoopT.
 
+Module LayerImplLoop.
+  Export LayerImplLoopT.
+  Section S.
+    Context S
+            `(l1 : Layer O1 S)
+            `(l2 : Layer O2 S)
+            (a : LayerImplLoopT.t l1 l2).
 
-Module LayerImplLoop
-  (s : State)
-  (o1 : Ops) (l1 : Layer o1 s)
-  (o2 : Ops) (l2 : Layer o2 s)
-  (a : LayerImplLoopT s o1 l1 o2 l2) <: LayerImpl o1 s l1 o2 s l2.
+    Definition absR (s1 : S) (s2 : S) := s1 = s2.
 
-  Definition absR (s1 : s.State) (s2 : s.State) := s1 = s2.
+    Definition compile_ts ts :=
+      CompileLoop.compile_ts a.(compile_op) ts.
 
-  Definition compile_ts ts :=
-    CompileLoop.compile_ts a.compile_op ts.
+    Theorem compile_ts_no_atomics :
+      forall ts,
+        no_atomics_ts ts ->
+        no_atomics_ts (compile_ts ts).
+    Proof.
+      eapply CompileLoop.compile_ts_no_atomics.
+    Qed.
 
-  Theorem compile_ts_no_atomics :
-    forall ts,
-      no_atomics_ts ts ->
-      no_atomics_ts (compile_ts ts).
-  Proof.
-    eapply CompileLoop.compile_ts_no_atomics.
-  Qed.
+    Theorem absInitP :
+      forall s1,
+        l1.(initP) s1 ->
+        exists s2, absR s1 s2 /\
+                   l2.(initP) s2.
+    Proof.
+      unfold absR; eauto using a.(initP_compat).
+    Qed.
 
-  Theorem absInitP :
-    forall s1,
-      l1.initP s1 ->
-      exists s2, absR s1 s2 /\
-      l2.initP s2.
-  Proof.
-    unfold absR; eauto using a.initP_compat.
-  Qed.
+    Theorem compile_traces_match :
+      forall ts,
+        no_atomics_ts ts ->
+        traces_match_abs absR l1.(initP) l2.(initP) l1.(step) l2.(step) (compile_ts ts) ts.
+    Proof.
+      unfold traces_match_abs, absR; intros; subst.
+      init_abs.
+      intuition auto using a.(initP_compat).
+      eapply CompileLoop.compile_traces_match_ts; eauto.
+      eapply a.(noop_or_success).
+      eapply CompileLoop.compile_ts_ok; eauto.
+    Qed.
 
-  Theorem compile_traces_match :
-    forall ts,
-      no_atomics_ts ts ->
-      traces_match_abs absR l1.initP l2.initP l1.step l2.step (compile_ts ts) ts.
-  Proof.
-    unfold traces_match_abs, absR; intros; subst.
-    init_abs.
-    intuition auto using a.initP_compat.
-    eapply CompileLoop.compile_traces_match_ts; eauto.
-    eapply a.noop_or_success.
-    eapply CompileLoop.compile_ts_ok; eauto.
-  Qed.
-
+  End S.
 End LayerImplLoop.
-
 
 (** General layer transformers. *)
 
-Module Link
-  (oA : Ops) (sA : State) (a : Layer oA sA)
-  (oB : Ops) (sB : State) (b : Layer oB sB)
-  (oC : Ops) (sC : State) (c : Layer oC sC)
-  (x : LayerImpl oA sA a oB sB b)
-  (y : LayerImpl oB sB b oC sC c) <: LayerImpl oA sA a oC sC c.
+Module Link.
+  Import LayerImpl.
+  Section S.
+    Context
+      `(a: Layer OA SA)
+      `(b: Layer OB SB)
+      `(c: Layer OC SC)
+      (x: LayerImpl.t a b)
+      (y: LayerImpl.t b c).
+    
+    Definition link_absR (s1 : SA) (s3 : SC) :=
+      exists s2, x.(absR) s1 s2 /\ y.(absR) s2 s3.
 
-  Definition absR (s1 : sA.State) (s3 : sC.State) :=
-    exists s2, x.absR s1 s2 /\ y.absR s2 s3.
+    Definition compile_ts ts :=
+      x.(compile_ts) (y.(compile_ts) ts).
 
-  Definition compile_ts ts :=
-    x.compile_ts (y.compile_ts ts).
+    Check compile_ts.
+    Theorem link_compile_ts_no_atomics :
+      forall ts,
+        no_atomics_ts ts ->
+        no_atomics_ts (compile_ts ts).
+    Proof.
+      intros.
+      eapply x.(compile_ts_no_atomics).
+      eapply y.(compile_ts_no_atomics).
+      eauto.
+    Qed.
 
-  Theorem compile_ts_no_atomics :
-    forall ts,
-      no_atomics_ts ts ->
-      no_atomics_ts (compile_ts ts).
-  Proof.
-    intros.
-    eapply x.compile_ts_no_atomics.
-    eapply y.compile_ts_no_atomics.
-    eauto.
-  Qed.
+    Theorem absInitP :
+      forall s1,
+        a.(initP) s1 ->
+        exists s2, link_absR s1 s2 /\ c.(initP) s2.
+    Proof.
+      unfold link_absR; intros.
+      eapply x.(absInitP) in H; propositional.
+      eapply y.(absInitP) in H0; propositional.
+      eauto.
+    Qed.
 
-  Theorem absInitP :
-    forall s1,
-      a.initP s1 ->
-      exists s2, absR s1 s2 /\ c.initP s2.
-  Proof.
-    unfold absR; intros.
-    eapply x.absInitP in H; propositional.
-    eapply y.absInitP in H0; propositional.
-    eauto.
-  Qed.
+    Lemma absR_transitive : forall s1 s2 s3,
+        x.(absR) s1 s2 ->
+        y.(absR) s2 s3 ->
+        link_absR s1 s3.
+    Proof.
+      unfold link_absR; eauto.
+    Qed.
 
-  Hint Resolve x.compile_ts_no_atomics y.compile_ts_no_atomics.
+    Hint Resolve absR_transitive.
 
-  Lemma absR_transitive : forall s1 s2 s3,
-      x.absR s1 s2 ->
-      y.absR s2 s3 ->
-      absR s1 s3.
-  Proof.
-    unfold absR; eauto.
-  Qed.
+    Theorem compile_traces_match :
+      forall ts,
+        no_atomics_ts ts ->
+        traces_match_abs link_absR a.(initP) c.(initP) a.(step) c.(step) (compile_ts ts) ts.
+    Proof.
+      unfold traces_match_abs; intros.
+      eapply x.(compile_traces_match) in H1; propositional; eauto.
+      eapply y.(compile_traces_match) in H3; propositional; eauto.
+      eapply y.(compile_ts_no_atomics); eauto.
+    Qed.
 
-  Hint Resolve absR_transitive.
-
-  Theorem compile_traces_match :
-    forall ts,
-      no_atomics_ts ts ->
-      traces_match_abs absR a.initP c.initP a.step c.step (compile_ts ts) ts.
-  Proof.
-    unfold traces_match_abs; intros.
-    eapply x.compile_traces_match in H1; propositional; eauto.
-    eapply y.compile_traces_match in H3; propositional; eauto.
-  Qed.
-
+  End S.
 End Link.
